theories/IL/Subterm.v
@@ -1,30 +1,120 @@
-Require Import List IL.
+Require Import List IL DecSolve.
 
 Set Implicit Arguments.
 
-Inductive subTerm : stmt -> stmt -> Prop :=
-| subTerm_refl s : subTerm s s
-| subTermExp s x e s' : subTerm s s' -> subTerm s (stmtLet x e s')
-| subTermIf1 e s s' t : subTerm s s' -> subTerm s (stmtIf e s' t)
-| subTermIf2 e s t t' : subTerm t t' -> subTerm t (stmtIf e s t')
-| subTermLet1 F t t' : subTerm t t' -> subTerm t (stmtFun F t')
-| subTermLet2 s Zs F t n : get F n Zs -> subTerm s (snd Zs) -> subTerm s (stmtFun F t).
+Inductive subTermInd : stmt -> stmt -> Prop :=
+| subTermInd_refl s : subTermInd s s
+| subTermIndExp s x e s' : subTermInd s s' -> subTermInd s (stmtLet x e s')
+| subTermIndIf1 e s s' t : subTermInd s s' -> subTermInd s (stmtIf e s' t)
+| subTermIndIf2 e s t t' : subTermInd t t' -> subTermInd t (stmtIf e s t')
+| subTermIndLet1 F t t' : subTermInd t t' -> subTermInd t (stmtFun F t')
+| subTermIndLet2 s Zs F t n : get F n Zs -> subTermInd s (snd Zs) -> subTermInd s (stmtFun F t).
 
-Instance subTerm_refl' : Reflexive subTerm.
+Instance eq_dec_pair A B  `{EqDec A eq} `{EqDec B eq} : EqDec (A*B) eq.
 Proof.
-  hnf; intros. eapply subTerm_refl.
+  hnf; intros [] []; unfold equiv, complement.
+  decide (a = a0); try dec_solve; subst.
+  decide (b = b0); try dec_solve; subst.
+  left. eauto.
+Defined.
+
+Instance eq_dec_pair_inst A B (x y: A*B) `{Computable (fst x = fst y)}
+         `{Computable (snd x = snd y)} : Computable (x = y).
+Proof.
+  destruct x,y; simpl in *.
+  decide (a = a0); try dec_solve; subst.
+  decide (b = b0); try dec_solve; subst.
+  left. eauto.
+Defined.
+
+Ltac decide_tac_rec P :=
+  first [ destruct (@decision_procedure P _)
+        | let X := fresh "C" in
+          first [ assert (X:Computable(P))
+                  by eauto 20 using get with typeclass_instances;
+                  destruct (@decision_procedure P X)
+                | let P' := eval symmetry in P in
+                      assert (X:Computable(P'))
+                    by eauto 20 using get with typeclass_instances;
+                                            destruct (@decision_procedure P' X)
+                ]
+        ].
+
+Tactic Notation "rdecide" constr(P) := decide_tac_rec P.
+
+Ltac eq_decide :=
+    match goal with
+  | [ |- {?f ?a ?b ?c = ?f ?a' ?b' ?c'} + {?f ?a ?b ?c <> ?f ?a' ?b' ?c'} ]
+    => try rdecide (a = a'); try rdecide (b = b'); try rdecide (c = c'); subst;
+        try dec_solve
+  | [ |- {?f ?a ?b = ?f ?a' ?b'} + {?f ?a ?b <> ?f ?a' ?b'} ]
+    => try rdecide (a = a'); try rdecide (b = b'); subst; try dec_solve
+  | [ |- {?f ?a = ?f ?a'} + {?f ?a <> ?f ?a'} ]
+    => try rdecide (a = a'); subst; try dec_solve
+  end.
+
+
+Instance list_equal_computable X
+  : forall (L L':list X), (forall n x x', get L n x -> get L' n x' -> Computable (x = x'))
+                     -> Computable (eq L L').
+Proof.
+  intros. decide (length L = length L').
+  - general induction L; destruct L'; isabsurd; try dec_solve.
+    rdecide (a = x); try dec_solve.
+    edestruct IHL with (L':=L'); eauto using get; subst; try dec_solve.
+  - right; intro; subst. eauto.
 Qed.
 
-Instance subTerm_trans : Transitive subTerm.
+Instance stmt_eq_dec (s t:stmt) : Computable (s = t).
+  revert t; sind s; intros;
+    destruct s, t; try dec_solve; hnf; try eq_decide.
+Qed.
+
+Instance exists_in_set_computable X (L:list X) (P:X->Prop)
+         `{forall n x, get L n x -> Computable (P x)}
+  : Computable (exists n x, get L n x /\ P x).
+Proof.
+  general induction L.
+  - dec_solve.
+  - rdecide (P a).
+    + left. eauto using get.
+    + edestruct IHL; dcr; eauto using get.
+      * left. dcr. do 2 eauto using get.
+      * right. intro. dcr. inv H1; eauto.
+Qed.
+
+
+Lemma subTermInd_dec s t : Computable (subTermInd s t).
+Proof.
+  revert s.
+  sind t; intros; decide (s = t); subst; try dec_solve; destruct t; simpl in *.
+  - edestruct (IH t); eauto; dec_solve.
+  - edestruct (IH t1); eauto; try dec_solve.
+    edestruct (IH t2); eauto; try dec_solve.
+  - dec_solve.
+  - dec_solve.
+  - rdecide (subTermInd s t); try dec_solve.
+    rdecide (exists n x, get F n x /\ subTermInd s (snd x)).
+    + left. destruct e as [? [? ?]]; dcr.
+      eauto using subTermInd.
+    + right. intro A; inv A; eauto.
+Qed.
+
+
+Instance subTermInd_refl' : Reflexive subTermInd.
+Proof.
+  hnf; intros. eapply subTermInd_refl.
+Qed.
+
+Instance subTermInd_trans : Transitive subTermInd.
 Proof.
   hnf; intros s t u ST1 ST2.
   general induction ST1; eauto;
-  general induction ST2; eauto using subTerm.
+  general induction ST2; eauto using subTermInd.
 Qed.
 
-
-Lemma subTerm_occurVars s t
-  : subTerm s t
+Lemma subTermInd_occurVars s t
+  : subTermInd s t
     -> occurVars s ⊆ occurVars t.
 Proof.
   intros. general induction H; simpl; eauto with cset.
@@ -33,12 +123,53 @@ Proof.
     eauto with cset.
 Qed.
 
+Lemma subTermIndF_occurVars F t sT
+  : subTermInd (stmtFun F t) sT
+    -> list_union (of_list ⊝ fst ⊝ F) ⊆ occurVars sT.
+Proof.
+  intros. general induction H; simpl.
+  - eapply list_union_incl; intros; eauto with cset.
+    inv_get.
+    rewrite <- incl_list_union; eauto using map_get_1.
+    cset_tac. cset_tac.
+  - rewrite IHsubTermInd; eauto. cset_tac.
+  - rewrite IHsubTermInd; eauto. cset_tac.
+  - rewrite IHsubTermInd; eauto. cset_tac.
+  - rewrite IHsubTermInd; eauto.
+  - rewrite IHsubTermInd; eauto.
+    rewrite <- incl_list_union; eauto using map_get_1.
+    instantiate (1:=occurVars (snd Zs)). cset_tac. cset_tac.
+Qed.
+
+Definition subTerm (s t:stmt) := sumbool_bool (subTermInd_dec s t) = true.
+
+Require Import Coq.Logic.Eqdep_dec.
+
+Lemma subTerm_PI s t (p1 p2:subTerm s t)
+  : p1 = p2.
+Proof.
+  unfold subTerm in *.
+  eapply dec_UIP.
+  eapply bool_eqdec.
+Qed.
+
+Lemma sTI_sT s sT
+  : (sumbool_bool (subTermInd_dec s sT) = true) <-> subTermInd s sT.
+Proof.
+  split; intros.
+  - destruct (subTermInd_dec s sT); eauto; isabsurd.
+  - destruct (subTermInd_dec s sT); eauto; isabsurd.
+Qed.
+
+Ltac sTE :=  unfold subTerm in *; rewrite sTI_sT in *.
+
 Lemma subTerm_EQ_Let sT st x e s
   (EQ:st = stmtLet x e s)
   (ST:subTerm st sT)
   : subTerm s sT.
 Proof.
-  subst st. etransitivity; eauto. econstructor; reflexivity.
+  subst st; sTE.
+  etransitivity; eauto. econstructor; reflexivity.
 Qed.
 
 Lemma subTerm_EQ_If1 sT st x s t
@@ -46,7 +177,7 @@ Lemma subTerm_EQ_If1 sT st x s t
   (ST:subTerm st sT)
   : subTerm s sT.
 Proof.
-  subst st. etransitivity; eauto. econstructor; reflexivity.
+  subst st; sTE; etransitivity; eauto. econstructor; reflexivity.
 Qed.
 
 Lemma subTerm_EQ_If2 sT st x s t
@@ -54,7 +185,7 @@ Lemma subTerm_EQ_If2 sT st x s t
   (ST:subTerm st sT)
   : subTerm t sT.
 Proof.
-  subst st. etransitivity; eauto. econstructor; reflexivity.
+  subst st; sTE; etransitivity; eauto. econstructor; reflexivity.
 Qed.
 
 Lemma subTerm_EQ_Fun1 sT st F t
@@ -62,8 +193,8 @@ Lemma subTerm_EQ_Fun1 sT st F t
   (ST:subTerm st sT)
   : subTerm t sT.
 Proof.
-  intros. subst. etransitivity; eauto.
-  eapply subTermLet1; eauto. reflexivity.
+  intros. sTE. subst. etransitivity; eauto.
+  eapply subTermIndLet1; eauto. reflexivity.
 Qed.
 
 Lemma subTerm_EQ_Fun2 sT st F t
@@ -71,15 +202,28 @@ Lemma subTerm_EQ_Fun2 sT st F t
   (ST:subTerm st sT)
   : forall (n : nat) (s : params * stmt), get F n s -> subTerm (snd s) sT.
 Proof.
-  intros. subst. etransitivity; eauto.
-  eapply subTermLet2; eauto. reflexivity.
+  intros. sTE. subst. etransitivity; eauto.
+  eapply subTermIndLet2; eauto. reflexivity.
 Qed.
 
-Require Import ProofIrrelevance.
-
-Lemma subTerm_PI s s'
-      (p p':subTerm s s')
-  : p = p'.
+Lemma subTerm_occurVars s t
+  : subTerm s t
+    -> occurVars s ⊆ occurVars t.
 Proof.
-  eapply proof_irrelevance.
+  intros. sTE.
+  eapply subTermInd_occurVars; eauto.
+Qed.
+
+Lemma subTerm_refl s
+  : subTerm s s.
+Proof.
+  sTE. econstructor.
+Qed.
+
+Lemma subTermF_occurVars F t sT
+  : subTerm (stmtFun F t) sT
+    -> list_union (of_list ⊝ fst ⊝ F) ⊆ occurVars sT.
+Proof.
+  sTE. intros.
+  eapply subTermIndF_occurVars; eauto.
 Qed.
